examples/machine-code/compiler/codegen_inputLib.sml
@@ -47,9 +47,9 @@ datatype assign_exp_type =
 
 datatype assign_type = 
     ASSIGN_EXP of int * assign_exp_type        (* register := expression *)
-  | ASSIGN_STACK of int * int                  (* stack[offset] := register *)
-  | ASSIGN_MEMORY of access_type * assign_address_type * int 
-                                               (* mem[address] := register *)
+  | ASSIGN_STACK of int * assign_x_type        (* stack[offset] := x *)
+  | ASSIGN_MEMORY of access_type * assign_address_type * assign_x_type
+                                               (* mem[address] := x *)
   | ASSIGN_OTHER of term * term                (* lhs := rhs *);
 
 datatype guard_compare_type =
@@ -60,20 +60,29 @@ datatype guard_compare_type =
 datatype guard_type =
     GUARD_NOT of guard_type
   | GUARD_COMPARE of int * guard_compare_type * assign_x_type  (* reg, cmp, reg/const *)
+  | GUARD_EQUAL_BYTE of assign_address_type * Arbnum.num 
   | GUARD_TEST of int * assign_x_type
   | GUARD_OTHER of term;
 
 
 (* term2guard, term2assign *)
 
+fun dest_var_char c tm = 
+  if not ((hd o explode o fst o dest_var) tm = c) then hd [] else
+    (string_to_int o implode o tl o explode o fst o dest_var) tm
+val dest_reg = dest_var_char #"r"
+val dest_stack = dest_var_char #"s"
+fun dest_n2w tm = if car tm = ``n2w:num->word32`` then numSyntax.dest_numeral (cdr tm) else hd []
+fun dest_n2w_byte tm = if car tm = ``n2w:num->word8`` then numSyntax.dest_numeral (cdr tm) else hd []
+fun dest_x tm = ASSIGN_X_REG (dest_reg tm) handle e => ASSIGN_X_CONST (dest_n2w tm)
+fun dest_address tm = ASSIGN_ADDRESS_REG (dest_reg tm) handle e =>
+  (if not ((fst o dest_const o car o car) tm = "word_add") then hd [] else
+    ASSIGN_ADDRESS_OFFSET_ADD ((dest_reg o cdr o car) tm, dest_n2w (cdr tm))) handle e =>
+  if not ((fst o dest_const o car o car) tm = "word_sub") then hd [] else
+    ASSIGN_ADDRESS_OFFSET_SUB ((dest_reg o cdr o car) tm, dest_n2w (cdr tm))
+
 fun basic_term2guard tm = (* expects input to use "~", "<+", "<" and "=" only *)
   if can dest_neg tm then GUARD_NOT (basic_term2guard (dest_neg tm)) else let
-    fun dest_var_char c tm = 
-      if not ((hd o explode o fst o dest_var) tm = c) then hd [] else
-        (string_to_int o implode o tl o explode o fst o dest_var) tm
-    val dest_reg = dest_var_char #"r"
-    fun dest_n2w tm = if car tm = ``n2w:num->word32`` then numSyntax.dest_numeral (cdr tm) else hd []
-    fun dest_x tm = ASSIGN_X_REG (dest_reg tm) handle e => ASSIGN_X_CONST (dest_n2w tm)
     val cmps = [("word_lo", (GUARD_COMPARE_LESS false, GUARD_COMPARE_LESS_EQUAL false)), 
                 ("word_lt", (GUARD_COMPARE_LESS true, GUARD_COMPARE_LESS_EQUAL true)), 
                 ("=", (GUARD_COMPARE_EQUAL, GUARD_COMPARE_EQUAL))] 
@@ -85,7 +94,14 @@ fun basic_term2guard tm = (* expects input to use "~", "<+", "<" and "=" only *)
        else if can dest_n2w x1 then 
          GUARD_NOT (GUARD_COMPARE (dest_reg x2, d2, dest_x x1))
        else 
-         GUARD_COMPARE (dest_reg x1, d1, dest_x x2) handle e =>
+         GUARD_COMPARE (dest_reg x1, d1, dest_x x2) 
+       handle e => let
+         val (i,_) = match_term ``(f:word32->word8) a = n2w n`` tm handle e =>
+                     match_term ``n2w n = (f:word32->word8) a`` tm
+         val addr = dest_address (subst i ``a:word32``)        
+         val imm = dest_n2w_byte (subst i ``(n2w n):word8``)        
+         in GUARD_EQUAL_BYTE (addr,imm) end        
+       handle e =>
          GUARD_OTHER tm
     end;
 
@@ -97,18 +113,6 @@ fun term2guard tm = let
   in f (basic_term2guard tm) end;
 
 fun basic_term2assign t1 t2 = let
-  fun dest_var_char c tm = 
-    if not ((hd o explode o fst o dest_var) tm = c) then hd [] else
-      (string_to_int o implode o tl o explode o fst o dest_var) tm
-  val dest_reg = dest_var_char #"r"
-  val dest_stack = dest_var_char #"s"
-  fun dest_n2w tm = if car tm = ``n2w:num->word32`` then numSyntax.dest_numeral (cdr tm) else hd []
-  fun dest_x tm = ASSIGN_X_REG (dest_reg tm) handle e => ASSIGN_X_CONST (dest_n2w tm)
-  fun dest_address tm = ASSIGN_ADDRESS_REG (dest_reg tm) handle e =>
-    (if not ((fst o dest_const o car o car) tm = "word_add") then hd [] else
-      ASSIGN_ADDRESS_OFFSET_ADD ((dest_reg o cdr o car) tm, dest_n2w (cdr tm))) handle e =>
-    if not ((fst o dest_const o car o car) tm = "word_sub") then hd [] else
-      ASSIGN_ADDRESS_OFFSET_SUB ((dest_reg o cdr o car) tm, dest_n2w (cdr tm))
   val binops = [("word_add",ASSIGN_BINOP_ADD), ("word_sub",ASSIGN_BINOP_SUB),
                 ("word_mul",ASSIGN_BINOP_MUL), ("word_and",ASSIGN_BINOP_AND),
                 ("word_div",ASSIGN_BINOP_DIV), ("word_mod",ASSIGN_BINOP_MOD),
@@ -138,8 +142,10 @@ fun basic_term2assign t1 t2 = let
       ((dest_x o cdr o car) tm, (Arbnum.toInt o numSyntax.dest_numeral o cdr) tm)
   fun dest_memory_update tm = 
     if not (is_var (cdr tm) andalso (fst o dest_const o car o car o car) tm = "UPDATE") 
-    then hd [] else (ACCESS_WORD, (dest_address o cdr o car o car) tm, (dest_reg o cdr o car) tm)
-    handle e => (ACCESS_BYTE, (dest_address o cdr o car o car) tm, (dest_reg o cdr o cdr o car) tm)
+    then hd [] else (ACCESS_WORD, (dest_address o cdr o car o car) tm, (dest_x o cdr o car) tm)
+    handle e => (ACCESS_BYTE, (dest_address o cdr o car o car) tm, 
+                 (dest_x o cdr o cdr o car) tm 
+                 handle e => (ASSIGN_X_CONST o dest_n2w_byte o cdr o car) tm)
   in ASSIGN_EXP (dest_reg t1, ASSIGN_EXP_REG (dest_reg t2)) handle e =>
      ASSIGN_EXP (dest_reg t1, ASSIGN_EXP_CONST (dest_n2w t2)) handle e =>
      ASSIGN_EXP (dest_reg t1, ASSIGN_EXP_STACK (dest_stack t2)) handle e =>
@@ -150,7 +156,7 @@ fun basic_term2assign t1 t2 = let
      ASSIGN_EXP (dest_reg t1, ASSIGN_EXP_SHIFT_LEFT (dest_lsl t2)) handle e =>
      ASSIGN_EXP (dest_reg t1, ASSIGN_EXP_SHIFT_RIGHT (dest_lsr t2)) handle e =>
      ASSIGN_EXP (dest_reg t1, ASSIGN_EXP_SHIFT_ARITHMETIC_RIGHT (dest_asr t2)) handle e =>
-     ASSIGN_STACK (dest_stack t1, dest_reg t2) handle e =>
+     ASSIGN_STACK (dest_stack t1, dest_x t2) handle e =>
      ASSIGN_MEMORY (dest_memory_update t2) handle e =>
      ASSIGN_OTHER (t1,t2)
   end
