examples/machine-code/hoare-triple/prog_x86Lib.sml
@@ -3,8 +3,9 @@ struct
  
 open HolKernel boolLib bossLib;
 open wordsLib stringLib addressTheory pred_setTheory combinTheory;
-open set_sepTheory x86_Theory x86_Lib prog_x86Theory helperLib;
-open x86_seq_monadTheory x86_coretypesTheory x86_astTheory;
+open set_sepTheory x86_Theory x86_Lib helperLib;
+open x86_seq_monadTheory x86_coretypesTheory x86_astTheory x86_icacheTheory;
+open prog_x86Theory;
 
 infix \\ 
 val op \\ = op THEN;
@@ -12,61 +13,80 @@ val op \\ = op THEN;
 
 val x86_status = xS_HIDE;
 val x86_pc = ``xPC``;
+val x86_exec_flag = ref false;
+val x86_code_write_perm = ref false;
+fun set_x86_exec_flag b = (x86_exec_flag := b);
+fun set_x86_code_write_perm_flag b = (x86_code_write_perm := b);
 
-fun process v tm = let
-  fun replace_plus c = if c = #"+" then #"_" else c;
-  fun name_of_tm tm = 
-    "m_" ^ (implode o filter is_normal_char o map replace_plus o explode o term_to_string) tm;
+fun name_for_resource counter tm = let
   val to_lower_drop_two = implode o tl o tl o explode o to_lower
-  in if type_of tm = ``:Xreg`` then 
-       (mk_comb(``xR``,tm),mk_var((to_lower o fst o dest_const) tm,``:word32``))
-     else if type_of tm = ``:Xeflags`` then 
-       (mk_comb(``xS1``,tm),mk_var((to_lower_drop_two o fst o dest_const) tm,``:bool option``))
-     else if type_of tm = ``:word32`` then
-       (mk_comb(``xM1``,tm),v)
-     else hd [] end;
+  in if type_of tm = ``:Xreg`` then (to_lower o fst o dest_const) tm else 
+     if type_of tm = ``:Xeflags`` then (to_lower_drop_two o fst o dest_const) tm else
+     (counter := 1 + !counter; ("x" ^ int_to_string (!counter))) end;
 
 fun pre_process_thm th = let
-  val rs = find_terml (can (match_term ``XREAD_REG x s``)) (concl th)
-  val fs = find_terml (can (match_term ``XREAD_EFLAG x s``)) (concl th)
-  val regs = map (fn tm => mk_eq(tm,(snd o process T o cdr o car) tm)) rs
-  fun f t = optionSyntax.mk_some o (fn x => mk_var(x,t)) o fst o dest_var
-  val flags = map (fn tm => mk_eq(tm,(f ``:bool`` o snd o process T o cdr o car) tm)) fs
-  val th = foldr (uncurry DISCH) th (regs @ flags @ [``XREAD_EIP s = eip``])
-  val th = SIMP_RULE bool_ss [optionTheory.option_CLAUSES] th
-  val ms = find_terml (can (match_term ``~(XREAD_MEM x s = NONE)``)) (concl th)
-  val ms = map (fst o dest_eq o dest_neg) ms
-  val mems = map (fn tm => mk_eq(tm,f ``:word8`` (genvar(``:bool``)))) ms
-  val th = foldr (uncurry DISCH) th mems
+  val x = ref 0
+  fun all_distinct [] = [] 
+    | all_distinct (x::xs) = x :: all_distinct (filter (fn y => not (x = y)) xs)
+  val rs = find_terml (fn tm => type_of tm = ``:Xreg``) (concl th)
+  val fs = find_terml (fn tm => type_of tm = ``:Xeflags``) (concl th)
+  val ws = find_terml (can (match_term ``XREAD_MEM2_WORD a``)) (concl th)
+  val ws = ws @ find_terml (can (match_term ``XWRITE_MEM2_WORD a``)) (concl th)
+  val ws = all_distinct (map cdr ws)
+  val bs = find_terml (can (match_term ``XREAD_MEM2 a``)) (concl th)
+  val bs = bs @ find_terml (can (match_term ``XWRITE_MEM2 a``)) (concl th)
+  val bs = all_distinct (map cdr bs)
+  fun make_eq_tm pattern lhs name = let
+    val var = mk_var(name_for_resource x name, type_of pattern)
+    in mk_eq(subst [lhs |-> name] pattern,var) end
+  val rs2 = map (make_eq_tm ``XREAD_REG r s`` ``r:Xreg``) rs
+  val fs2 = map (make_eq_tm ``XREAD_EFLAG f s`` ``f:Xeflags``) fs
+  val ws2 = map (make_eq_tm ``XREAD_MEM2_WORD a s`` ``a:word32``) ws
+  val bs2 = map (make_eq_tm ``XREAD_MEM2 a s`` ``a:word32``) bs
+  val result = rs2 @ fs2 @ ws2 @ bs2 @ [``XREAD_EIP s = eip``]   
+  val th = foldr (uncurry DISCH) th result
   val th = RW [AND_IMP_INTRO,GSYM CONJ_ASSOC,wordsTheory.WORD_XOR_CLAUSES,
-             wordsTheory.WORD_AND_CLAUSES] (SIMP_RULE std_ss [] th)
+             wordsTheory.WORD_AND_CLAUSES,wordsTheory.WORD_ADD_0] (SIMP_RULE std_ss [] th)
   in th end;
 
 fun x86_pre_post g s = let
   val h = g
-  val regs = collect_term_of_type ``:Xreg`` g;
-  val bits = collect_term_of_type ``:Xeflags`` g;
-  val mems = find_terml (can (match_term ``(XREAD_MEM x s = SOME y)``)) h
-  val mems = filter (is_var o cdr o cdr) mems
-  val mems = map (fn tm => ((cdr o car o fst o dest_eq) tm, cdr tm)) mems
-  val assignments = find_terml (can (match_term ``XWRITE_EFLAG a x``)) h
-                  @ find_terml (can (match_term ``XWRITE_REG a x``)) h
-                  @ find_terml (can (match_term ``XWRITE_MEM a x``)) h
-  val assignments = map (fn tm => (cdr (car tm) handle e => ``EIP``, cdr tm)) assignments  
+  val xs = find_terml (can (match_term ``(XREAD_REG x s = y)``)) h
+         @ find_terml (can (match_term ``(XREAD_MEM2_WORD x s = y)``)) h
+         @ find_terml (can (match_term ``(XREAD_MEM2 x s = y)``)) h
+         @ find_terml (can (match_term ``(XREAD_EFLAG x s = y)``)) h
+  val xs = map (fn tm => ((cdr o car o cdr o car) tm, cdr tm)) xs
+  val ys = find_terml (can (match_term ``XWRITE_EFLAG a x``)) h
+         @ find_terml (can (match_term ``XWRITE_MEM2 a x``)) h
+         @ find_terml (can (match_term ``XWRITE_MEM2_WORD a x``)) h
+         @ find_terml (can (match_term ``XWRITE_REG a x``)) h
+  val ys = map (fn tm => ((cdr o car) tm, cdr tm)) ys
   val new_eip = (cdr o hd) (find_terml (can (match_term ``XWRITE_EIP e``)) h)
   fun assigned_aux x y [] = y
-    | assigned_aux x y ((q,z)::zs) = if x = q then z else assigned_aux x y zs
-  fun get_assigned_value x y = assigned_aux x y assignments
-  fun mk_pre_post_assertion (x,v) = let
-    val (y,z) = process v x
-    val q = get_assigned_value x z
-    in (mk_comb(y,z),mk_comb(y,q)) end   
-  val pre_post = map mk_pre_post_assertion (map (fn tm => (tm,T)) (regs @ bits) @ mems) 
+    | assigned_aux x y ((q,z)::zs) = if aconv x q then z else assigned_aux x y zs
+  fun get_assigned_value x y = assigned_aux x y ys
+  fun mk_pre_post_assertion (name,var) = let
+    val (pattern,name_tm,var_tm) =
+          if type_of name = ``:Xreg`` then 
+            (``xR a w``,``a:Xreg``,``w:word32``) 
+          else if type_of name = ``:Xeflags`` then 
+            (``xS1 a w``,``a:Xeflags``,``w:bool option``) 
+          else if type_of var = ``:word8`` then 
+            (``~(xM1 a (SOME (w,xDATA_PERM ex)))``,``a:word32``,``w:word8``) 
+          else if type_of var = ``:word32`` then 
+            (``xM a w``,``a:word32``,``w:word32``) else hd []
+    in (subst [name_tm|->name,var_tm|->var] pattern,
+        subst [name_tm|->name,var_tm|->get_assigned_value name var] pattern) end
+  val pre_post = map mk_pre_post_assertion xs
   val pre = list_mk_star (map fst pre_post) ``:x86_set -> bool``
   val post = list_mk_star (map snd pre_post) ``:x86_set -> bool``
   fun is_precond tm =
    (not (can (match_term ``XREAD_REG r s = v``) tm) andalso
-    not (can (match_term ``XREAD_MEM r s = v``) tm) andalso
+    not (can (match_term ``XREAD_MEM2 r s = v``) tm) andalso
+    not (can (match_term ``XREAD_MEM2_WORD r s = v``) tm) andalso
+    not (can (match_term ``CAN_XWRITE_MEM r s``) tm) andalso
+    not (can (match_term ``CAN_XREAD_MEM r s``) tm) andalso
+    not (can (match_term ``XREAD_INSTR r s = v``) tm) andalso
     not (can (match_term ``XREAD_EFLAG r s = v``) tm) andalso
     not (can (match_term ``XREAD_EIP s = v``) tm)) handle e => true
   val all_conds = (list_dest dest_conj o fst o dest_imp) h
@@ -84,24 +104,11 @@ fun x86_pre_post g s = let
 
 fun introduce_xMEMORY th = let
   val (_,p,c,q) = dest_spec(concl th)
-  val tm3 = find_term (can (match_term ``xM1 (x + 3w) y``)) p
-  val tm2 = find_term (can (match_term ``xM1 (x + 2w) y``)) p
-  val tm1 = find_term (can (match_term ``xM1 (x + 1w) y``)) p
-  val tm0 = find_term (can (match_term ``xM1 (x + 0w) y``)) p
-  val c = MOVE_OUT_CONV (car tm3) THENC MOVE_OUT_CONV (car tm2) THENC
-          MOVE_OUT_CONV (car tm1) THENC MOVE_OUT_CONV (car tm0) THENC STAR_REVERSE_CONV
+  val tm = find_term (can (match_term ``xM x y``)) p
+  val c = MOVE_OUT_CONV (car tm) THENC STAR_REVERSE_CONV
   val th = CONV_RULE (POST_CONV c THENC PRE_CONV c) th
-  val f = cdr o cdr
-  fun g th tm tm' = if is_var tm then INST [ tm |-> tm' ] th else th
-  val th = g th (f tm0) ``((7 >< 0) (w:word32)):word8``   
-  val th = g th (f tm1) ``((7 >< 0) ((w >> 8):word32)):word8``   
-  val th = g th (f tm2) ``((7 >< 0) ((w >> 16):word32)):word8``   
-  val th = g th (f tm3) ``((7 >< 0) ((w >> 24):word32)):word8``   
-  val h = REWRITE_RULE [GSYM STAR_ASSOC,x86_seq_monadTheory.word2bytes_thm,x86_seq_monadTheory.EL_thm] 
-  val th = MATCH_MP (h xMEMORY_INTRO) (h th)
-  val th = SIMP_RULE bool_ss [GSYM ALIGNED_def,SEP_CLAUSES] th
-  val th = REWRITE_RULE [GSYM progTheory.SPEC_MOVE_COND,ALIGNED_def,
-             STAR_ASSOC,bit_listTheory.bytes2word_thm] th
+  val th = MATCH_MP xMEMORY_INTRO (RW [GSYM STAR_ASSOC] th)
+  val th = RW [GSYM progTheory.SPEC_MOVE_COND,STAR_ASSOC] th  
   fun replace_access_in_pre th = let
     val (_,p,c,q) = dest_spec(concl th)
     val tm = find_term (can (match_term ``(a:'a =+ w:'b) f``)) p
@@ -113,15 +120,15 @@ fun introduce_xMEMORY th = let
   val th = replace_access_in_pre th
   in th end handle e => th;
 
-fun introduce_xBYTE_MEMORY th = let
+fun introduce_xBYTE_MEMORY_ANY th = let
   val (_,p,c,q) = dest_spec(concl th)
-  val tm0 = find_term (can (match_term ``xM1 x y``)) p
-  val c = MOVE_OUT_CONV (car tm0) THENC STAR_REVERSE_CONV
-  val th = CONV_RULE (POST_CONV c THENC PRE_CONV c) th
-  val f = cdr o cdr
-  val h = REWRITE_RULE [GSYM STAR_ASSOC,x86_seq_monadTheory.word2bytes_thm,x86_seq_monadTheory.EL_thm] 
-  val th = MATCH_MP (h xBYTE_MEMORY_INTRO) (h th)
-  val th = RW [wordsTheory.WORD_ADD_0,GSYM progTheory.SPEC_MOVE_COND] th
+  val tm1 = find_term (can (match_term ``xM1 x y``)) p
+  val tm2 = find_term (can (match_term ``xM1 x y``)) q
+  val c1 = MOVE_OUT_CONV tm1 THENC STAR_REVERSE_CONV
+  val c2 = MOVE_OUT_CONV tm2 THENC STAR_REVERSE_CONV
+  val th = CONV_RULE (POST_CONV c2 THENC PRE_CONV c1) th
+  val th = MATCH_MP xBYTE_MEMORY_ANY_INTRO (RW [GSYM STAR_ASSOC] th)
+  val th = RW [GSYM progTheory.SPEC_MOVE_COND,STAR_ASSOC] th  
   fun replace_access_in_pre th = let
     val (_,p,c,q) = dest_spec(concl th)
     val tm = find_term (can (match_term ``(a:'a =+ w:'b) f``)) p
@@ -131,12 +138,11 @@ fun introduce_xBYTE_MEMORY th = let
     val th = REWRITE_RULE [APPLY_UPDATE_ID] (INST [x |-> mk_comb(y,a)] th)
     in th end handle e => th
   val th = replace_access_in_pre th
-  val th = RW [STAR_ASSOC] th
   in th end handle e => th;
 
 fun calculate_length_and_jump th = let 
   val (_,_,c,q) = dest_spec (concl th)
-  val l = (length o fst o listSyntax.dest_list o cdr o cdr o car) c
+  val l = (length o fst o listSyntax.dest_list o cdr o car o cdr o cdr o car) c
   in
     let val v = find_term (can (match_term ``xPC (p + n2w n)``)) q
     in (th,l,SOME (0 + (numSyntax.int_of_term o cdr o cdr o cdr) v)) end 
@@ -150,68 +156,90 @@ fun post_process_thm th = let
   val th = SIMP_RULE (std_ss++sw2sw_ss++w2w_ss) [wordsTheory.word_mul_n2w,SEP_CLAUSES] th
   val th = CONV_RULE FIX_WORD32_ARITH_CONV th
   val th = introduce_xMEMORY th
-  val th = introduce_xBYTE_MEMORY th
+  val th = introduce_xBYTE_MEMORY_ANY th
   val th = SIMP_RULE (std_ss++sw2sw_ss++w2w_ss) [GSYM wordsTheory.WORD_ADD_ASSOC,
     word_arith_lemma1,word_arith_lemma2,word_arith_lemma3,word_arith_lemma4] th
   val th = CONV_RULE FIX_WORD32_ARITH_CONV th
   val th = RW [wordsTheory.WORD_ADD_ASSOC,wordsTheory.WORD_ADD_0] th
+  fun f th = let
+    val x = find_term (can (match_term ``(THE x):'a``)) (concl th)
+    val y = optionSyntax.mk_some(mk_var(fst (dest_var (cdr x)),type_of x))
+    val th = INST [cdr x |-> y] th
+    val th = SIMP_RULE (bool_ss++optionTheory.option_rwts) [SEP_CLAUSES] th
+    in th end
+  val th = repeat f th
+  val th = RW [ALIGNED_def] th
+  val th = SIMP_RULE std_ss [wordsTheory.WORD_EQ_SUB_ZERO,w2w_eq_n2w] th
   in calculate_length_and_jump th end;
 
-fun calc_code s = let
-  fun space n [] zs = [implode zs]
-    | space n (x::xs) zs = 
-        if n = 0 then (implode zs) :: space 2 (x::xs) [] else space (n-1) xs (zs @ [x])
-  fun get_rewrite c = GSYM (EVAL (subst [``c:string``|->fromMLstring c] ``hex2bits c``))
-  val strs = space 2 (explode s) []
-  val tm = ``(b2w I (hex2bits s)):word8``  
-  val zs = map (fn x => subst [``s:string``|-> fromMLstring x] tm) strs
-  val rws = map EVAL zs
-  val c = listSyntax.mk_list (map (cdr o concl) rws, ``:word8``)
-  in (c, map get_rewrite strs @ rws) end;  
+fun calc_code th = let
+  val tms = find_terml (can (match_term ``XREAD_INSTR a s = SOME x``)) (concl th)
+  val tms = map dest_eq tms
+  fun addr tm = (Arbnum.toInt o numSyntax.dest_numeral o cdr o cdr o cdr o car) tm
+                handle e => 0
+  val tms = map (fn (x,y) => (addr x, cdr y)) tms
+  val code = map snd (sort (fn (x,_) => fn (y,_) => x <= y) tms)
+  in listSyntax.mk_list (code, ``:word8``) end;
 
 fun x86_prove_one_spec th c = let
   val g = concl th
   val s = find_term (can (match_term ``X86_NEXT x = SOME y``)) g
   val s = (snd o dest_comb o snd o dest_comb) s    
   val (pre,post) = x86_pre_post g s
-  val tm = ``SPEC X86_MODEL pre {(eip,c)} post``
+  val tm = ``SPEC X86_MODEL pre {(eip,(c,w))} post``
   val tm = subst [mk_var("pre",type_of pre) |-> pre, 
                   mk_var("post",type_of post) |-> post, 
                   mk_var("c",type_of c) |-> c] tm
   val FLIP_TAC = CONV_TAC (ONCE_REWRITE_CONV [EQ_SYM_EQ])
-  val th1 = SIMP_RULE bool_ss [XWRITE_EIP_def,XWRITE_EFLAG_def,XWRITE_REG_def,XWRITE_MEM_def,
-    XREAD_REG_def,XREAD_MEM_def,XREAD_EFLAG_def,XREAD_EIP_def] (Q.INST [`s`|->`(xr,xf,xe,xm)`] th)
+  val th1 = Q.INST [`s`|->`X86_ICACHE_UPDATE x (r,e,t,m,i)`] th
+  val th1 = RW [XREAD_CLAUSES,XWRITE_MEM2_WORD_def] th1 
+  val th1 = RW [XWRITE_EFLAG_def,X86_ICACHE_UPDATE_def,XWRITE_MEM2_def,XWRITE_REG_def,
+        APPLY_UPDATE_THM,WORD_EQ_ADD_CANCEL,x86_address_lemma,XWRITE_EIP_def] th1
   val th = prove(tm,
 (*
     set_goal([],tm)
 *)
-    MATCH_MP_TAC IMP_X86_SPEC \\ REPEAT STRIP_TAC \\ EXISTS_TAC ((cdr o cdr o concl o UNDISCH) th1)
+    MATCH_MP_TAC IMP_X86_SPEC \\ REPEAT STRIP_TAC 
+    \\ EXISTS_TAC ((cdr o cdr o concl o UNDISCH) th1)
+    \\ STRIP_TAC \\ REWRITE_TAC [X86_ICACHE_UPDATE_def]
+    THENL [MATCH_MP_TAC th1,ALL_TAC]
+    \\ REPEAT (POP_ASSUM MP_TAC)
     \\ SIMP_TAC (std_ss++wordsLib.SIZES_ss) [GSYM STAR_ASSOC,
          STAR_x86_2set, IN_DELETE, APPLY_UPDATE_THM, Xreg_distinct,
          GSYM ALIGNED_def, wordsTheory.n2w_11, Xeflags_distinct,
          Q.SPECL [`s`,`x INSERT t`] SET_EQ_SUBSET, INSERT_SUBSET,
-         EMPTY_SUBSET, SEP_CLAUSES] 
+         EMPTY_SUBSET, SEP_CLAUSES,X86_ICACHE_UPDATE_def,XCLEAR_ICACHE_def,
+         X86_ICACHE_REVERT_def,xM_def,WORD_EQ_ADD_CANCEL,x86_address_lemma] 
     \\ ONCE_REWRITE_TAC [CODE_POOL_x86_2set]
     \\ REWRITE_TAC [listTheory.LENGTH,address_list_def]
-    \\ SIMP_TAC std_ss [arithmeticTheory.ADD1]
+    \\ SIMP_TAC std_ss [arithmeticTheory.ADD1,X86_ICACHE_EXTRACT_def]
     \\ SIMP_TAC (std_ss++wordsLib.SIZES_ss) [GSYM STAR_ASSOC,
          STAR_x86_2set, IN_DELETE, APPLY_UPDATE_THM, Xreg_distinct,
          GSYM ALIGNED_def, wordsTheory.n2w_11, Xeflags_distinct,
          Q.SPECL [`s`,`x INSERT t`] SET_EQ_SUBSET, INSERT_SUBSET,
-         EMPTY_SUBSET,x86_pool_def] 
+         EMPTY_SUBSET,x86_pool_def,X86_ACCURATE_CLAUSES] 
+    \\ SIMP_TAC std_ss [XREAD_REG_def,XREAD_EFLAG_def,XREAD_EIP_def]
     \\ NTAC 3 (FLIP_TAC \\ SIMP_TAC std_ss [GSYM AND_IMP_INTRO])
-    \\ FLIP_TAC \\ REWRITE_TAC [AND_IMP_INTRO, GSYM CONJ_ASSOC] 
-    \\ SIMP_TAC std_ss [] \\ FLIP_TAC \\ STRIP_TAC \\ STRIP_TAC 
-    THEN1 (FLIP_TAC \\ MATCH_MP_TAC (REWRITE_RULE [GSYM ALIGNED_def] th1) \\ 
-           FULL_SIMP_TAC std_ss [ALIGNED_def,word_arith_lemma1,CONTAINER_def,markerTheory.Abbrev_def])    
-    \\ FULL_SIMP_TAC std_ss [UPDATE_x86_2set'',word_arith_lemma1,ALIGNED_CLAUSES])
+    \\ SIMP_TAC std_ss [CAN_XREAD_MEM,CAN_XWRITE_MEM,IN_INSERT]
+    \\ SIMP_TAC std_ss [XREAD_MEM2_WORD_def,XREAD_MEM2_def,wordsTheory.WORD_ADD_0]    
+    \\ SIMP_TAC std_ss [bit_listTheory.bytes2word_thm,IN_xDATA_PERM]
+    THEN1 (SIMP_TAC std_ss [markerTheory.Abbrev_def]
+           \\ REPEAT STRIP_TAC \\ FLIP_TAC \\ MATCH_MP_TAC XREAD_INSTR_IMP 
+           \\ Q.EXISTS_TAC `w` \\ ASM_SIMP_TAC std_ss []
+           \\ FULL_SIMP_TAC std_ss [wordsTheory.word_add_n2w,GSYM wordsTheory.WORD_ADD_ASSOC])
+    \\ SIMP_TAC std_ss [word2bytes_thm,EL_thm,INSERT_SUBSET,IN_INSERT,EMPTY_SUBSET]
+    \\ FULL_SIMP_TAC std_ss [UPDATE_x86_2set'',word_arith_lemma1,
+         ALIGNED_CLAUSES,icache_revert_ID,X86_ACCURATE_UPDATE]
+    \\ SIMP_TAC std_ss [AND_IMP_INTRO]
+    \\ STRIP_TAC \\ IMP_RES_TAC X86_ACCURATE_IMP
+    \\ ASM_SIMP_TAC std_ss [] \\ FULL_SIMP_TAC std_ss [markerTheory.Abbrev_def])
+  val th = INST [``w:bool``|-> (if !x86_code_write_perm then T else F)] th
   in RW [STAR_ASSOC,SEP_CLAUSES,markerTheory.Abbrev_def] th end;
 
 fun x86_prove_specs s = let
   val th = x86_step s
+  val c = calc_code th
   val th = pre_process_thm th
-  val (c,thms) = calc_code s
-  val th = RW thms th
   fun replace_conv th tm = if (fst o dest_eq o concl) th = tm then th else ALL_CONV tm
   in if (is_cond o cdr o cdr o snd o dest_imp o concl) th then let
        val (x,y,z) = dest_cond (find_term is_cond (concl th))
@@ -229,10 +257,19 @@ fun x86_prove_specs s = let
 
 fun x86_jump (tm1:term) (tm2:term) (jump_length:int) (forward:bool) = ("",0)
 
-val x86_spec = cache x86_prove_specs;
+val x86_spec_aux = cache x86_prove_specs;
+fun x86_spec s = let
+  val ((th,i,j),other) = x86_spec_aux s
+  val b = if !x86_exec_flag then T else F
+  val th = INST [``ex:bool``|->b] th
+  val th = RW [GSYM xBYTE_MEMORY_def,GSYM xBYTE_MEMORY_X_def] th
+  in ((th,i,j),other) end
+
 val x86_tools = (x86_spec, x86_jump, x86_status, x86_pc)
 
 (*
+
+open x86_encodeLib;
 
   val th = x86_spec "40";              (* inc eax *)
   val th = x86_spec "F7C203000000";    (* test edx,3 *)
@@ -244,10 +281,6 @@ val x86_tools = (x86_spec, x86_jump, x86_status, x86_pc)
   val th = x86_spec "89CD";            (* mov ebp,ecx *)
   val th = x86_spec "45";              (* inc ebp *)
   val th = x86_spec "EBF7";            (* jmp L1 *)
-  val th = x86_spec "E2FD";            (* loop L *)
-  val th = x86_spec "751D";            (* jne L1 *)
-  val th = x86_spec "740D";            (* je L2 *)
-  val th = x86_spec "0F44C1";          (* cmove eax, ecx *)
   val th = x86_spec "8B36";            (* mov esi, [esi] *)
   val th = x86_spec "8B2A";            (* mov ebp,[edx] *)
   val th = x86_spec "8B7204";          (* mov esi,[edx+4] *)
@@ -259,7 +292,22 @@ val x86_tools = (x86_spec, x86_jump, x86_status, x86_pc)
   val th = x86_spec "F720";            (* mul dword [eax] *)
   val th = x86_spec "F7F6";            (* div esi *)
   val th = x86_spec "883E";            (* mov_byte [esi],edi *)
-  val th = x86_spec "8A3E";            (* mov_byte edi,[esi] *)
+  val th = x86_spec "0FB63E";          (* mov_byte edi,[esi] *)
+  val th = x86_spec "E2FD";            (* loop L *)
+  val th = x86_spec "751D";            (* jne L1 *)
+  val th = x86_spec "740D";            (* je L2 *)
+  val th = x86_spec "0F44C1";          (* cmove eax, ecx *)
+  val th = x86_spec (x86_encode "mov_byte [esi],-10")
+
+  val th = x86_spec "31C0";
+  val th = x86_spec "85F6";
+  val th = x86_spec "8B36";
+  val th = x86_spec "85F6";
+  val th = x86_spec "7405";
+
+  val th = x86_spec (x86_encode "jmp edx")
+
+  val th = x86_spec "E9";              (* jmp imm32 *)
 
 *)
 
