examples/machine-code/lisp/export_codeLib.sml
@@ -5,17 +5,13 @@ open HolKernel boolLib bossLib Parse;
 
 open wordsTheory wordsLib helperLib;
 
-open divideTheory;
-
-val filename = "foo"
-val th = arm_div_mod_thm
-
 fun write_code_to_file filename th = let
   val _ = print ("Extracting machine code to file \"" ^ filename ^ "\", ")
   val (m,pre,c,post) = (dest_spec o concl) th
   val model_name = fst (dest_const m)
   val cs = butlast (list_dest pred_setSyntax.dest_insert c)
   val vs = map (pairSyntax.dest_pair) cs
+  val vs = map (fn (x,y) => (x,fst (pairSyntax.dest_pair y) handle e => y)) vs
   val vs = map (fn (x,y) => (if is_var x then ``0:num`` else cdr (cdr x),y)) vs
   val vs = map (fn (x,y) => (Arbnum.toInt (numSyntax.dest_numeral x),y)) vs
   val vs = sort (fn (x,_) => fn (y:int,_) => x <= y) vs
@@ -23,17 +19,17 @@ fun write_code_to_file filename th = let
                                      x :: del_repetations (y::xs)
     | del_repetations zs = zs
   val vs = del_repetations vs
-  fun no_duplicates (x::y::xs) = if fst x = fst y then hd [] else no_duplicates (y::xs)
+  fun no_duplicates (x::y::xs) = if fst x = fst y then hd [] else no_duplicates (y::xs) 
     | no_duplicates _ = true
-  val _ = no_duplicates vs
-  fun term_byte_size tm =
+  val _ = no_duplicates vs 
+  fun term_byte_size tm = 
     if type_of tm = ``:word8`` then 1 else
     if type_of tm = ``:word32`` then 4 else
       foldr (fn (x,y) => x + y) 0 (map term_byte_size (fst (listSyntax.dest_list tm)))
   fun no_holes i [] = true
-    | no_holes i ((j,c)::xs) =
+    | no_holes i ((j,c)::xs) = 
        if i = j then no_holes (i + (term_byte_size c)) xs else hd []
-  val _ = no_holes 0 vs
+  val _ = no_holes 0 vs 
   val byte_count = ref 0;
   val big_endian_format = ``[(w2w ((w:word32) >>> 24)):word8;
                              (w2w ((w:word32) >>> 16)):word8;
@@ -45,25 +41,25 @@ fun write_code_to_file filename th = let
                                 (w2w ((w:word32) >>> 24)):word8]``
   val format_tm = if model_name = "PPC_MODEL" then big_endian_format else little_endian_format
   val vs = map (fn (x,y) => (x,(cdr o concl o EVAL o subst [``w:word32``|->y]) format_tm handle e => y)) vs
-  fun fill c d n s = if size s < n then fill c d n (c ^ s ^ d) else s
+  fun fill c d n s = if size s < n then fill c d n (c ^ s ^ d) else s 
   fun word2hex tm = let
     val _ = (byte_count := !byte_count + (if type_of tm = ``:word8`` then 1 else 4))
     val s = Arbnum.toHexString (numSyntax.dest_numeral (cdr tm))
     in "0x" ^ fill "0" "" (if type_of tm = ``:word8`` then 2 else
                            if type_of tm = ``:word32`` then 8 else hd []) s end
-  fun word2string tm = let
-    val (tms,ty) = if listSyntax.is_list tm
+  fun word2string tm = let 
+    val (tms,ty) = if listSyntax.is_list tm 
                    then listSyntax.dest_list tm
-                   else ([tm],type_of tm)
-    val str = if ty = ``:word8`` then "\t.byte\t" else
+                   else ([tm],type_of tm)           
+    val str = if ty = ``:word8`` then "\t.byte\t" else 
               if ty = ``:word32`` then "\t.word\t" else hd []
     fun foo [] = hd []
       | foo [x] = word2hex x ^ "\n"
-      | foo (x::y::ys) = word2hex x ^ ", " ^ foo (y::ys)
+      | foo (x::y::ys) = word2hex x ^ ", " ^ foo (y::ys)    
     in str ^ foo tms end
   val rs = map (word2string o snd) vs
   val instr_count = length rs
-  val size_count = (!byte_count)
+  val size_count = (!byte_count) 
   val l1 = "Machine code automatically extracted from a HOL4 theorem."
   val l2 = "The code consists of " ^ int_to_string instr_count ^ " instructions (" ^ int_to_string size_count ^ " bytes)."
   val l3 = "End of automatically extracted machine code."
@@ -72,11 +68,10 @@ fun write_code_to_file filename th = let
   val o3 = "\t/*  " ^ fill "" " " (size l1) l3 ^ "  */\n"
   val output = ["\n","\n",o1,o2,"\n"] @ rs @ ["\n",o3,"\n"]
   (* val _ = map print output *)
-  (* write to text file *)
-  val out = TextIO.openOut filename
-  fun writeline s = TextIO.output(out,s)
-  val _ = map writeline output
-  val _ = TextIO.closeOut(out)
+  (* write to text file *)  
+  val t = TextIO.openOut(filename) 
+  val _ = map (fn s => TextIO.output(t,s)) output 
+  val _ = TextIO.closeOut(t)
   val _ = print "done.\n"
   in () end;
 
