examples/machine-code/instruction-set-models/common/opmonScript.sml
@@ -1,6 +1,6 @@
 
 open HolKernel boolLib bossLib Parse;
-open optionTheory;
+open optionTheory wordsTheory listTheory;
 
 val _ = new_theory "opmon";
 
@@ -15,10 +15,8 @@ val option_then_def = Define `
   option_then f g x =  
     let m = f x in (if m = NONE then NONE else g (THE m))`;
 
-val _ = overload_on ("++",Term`$option_orelse`);
+val _ = overload_on ("++",Term`$option_orelse`); 
 val _ = overload_on (">>",Term`$option_then`);
-val _ = add_infix("++", 680,HOLgrammars.LEFT);
-val _ = add_infix(">>", 680,HOLgrammars.LEFT);
 
 val option_fail_def = Define `option_fail = \x. NONE`;
 
@@ -30,7 +28,7 @@ val option_do_def = Define `
 val option_try_def = Define `
   (option_try [] = option_fail) /\
   (option_try [t] = t) /\
-  (option_try (t1::t2::ts) = t1 ++ option_try (t2::ts))`;
+  (option_try (t1::t2::ts) = option_orelse t1 (option_try (t2::ts)))`;
 
 val option_apply_def = Define `
   option_apply x f = if x = NONE then NONE else f (THE x)`;
@@ -46,24 +44,26 @@ val option_then_assoc = store_thm("option_then_assoc",
   THEN REPEAT STRIP_TAC THEN Cases_on `x x'` THEN SRW_TAC [] []);
 
 val option_orelse_assoc = store_thm("option_orelse_assoc",
-  ``!x y z. (x ++ y) ++ z = x ++ (y ++ z)``,
+  ``!x y z. option_orelse (option_orelse x y) z = 
+            option_orelse x (option_orelse y z)``,
   SIMP_TAC std_ss [FUN_EQ_THM,option_orelse_def,LET_DEF]  
   THEN REPEAT STRIP_TAC THEN Cases_on `x x'` THEN SRW_TAC [] []);
 
 val option_orelse_SOME = store_thm("option_orelse_SOME",
   ``!f g h. 
-      (f ++ g) >> SOME o k = (f >> SOME o k) ++ (g >> SOME o k)``,
+      (option_orelse f g) >> SOME o k = option_orelse (f >> SOME o k) (g >> SOME o k)``,
   SIMP_TAC std_ss [FUN_EQ_THM,option_orelse_def,option_then_def,LET_DEF]  
   THEN REPEAT STRIP_TAC THEN Cases_on `f x`
   THEN ASM_SIMP_TAC std_ss []);
 
 val option_then_OVER_orelse = store_thm("option_then_OVER_orelse",
   ``!x:'a -> 'b option y:'b -> 'c option g. 
-      ((x >> y) ++ (x >> z) = x >> (y ++ z)) /\ 
-      (g ++ (x >> y) ++ (x >> z) = g ++ x >> (y ++ z)) /\ 
-      ((x >> y) ++ (x >> z) ++ g = x >> (y ++ z) ++ g) /\ 
-      (h ++ (x >> y) ++ (x >> z) ++ g = h ++ x >> (y ++ z) ++ g)``,
-  REPEAT STRIP_TAC THEN `x >> y ++ x >> z = x >> (y ++ z)` by 
+      (option_orelse (x >> y) (x >> z) = x >> (option_orelse y z)) /\ 
+      (option_orelse (option_orelse g (x >> y)) (x >> z) = option_orelse g (x >> (option_orelse y z))) /\ 
+      (option_orelse (x >> y) (option_orelse (x >> z) g) = option_orelse (x >> (option_orelse y z)) g) /\ 
+      (option_orelse h (option_orelse (x >> y) (option_orelse (x >> z) g)) = 
+       option_orelse h (option_orelse (x >> (option_orelse y z)) g))``,
+  REPEAT STRIP_TAC THEN `option_orelse (x >> y) (x >> z) = x >> (option_orelse y z)` by 
     (SIMP_TAC std_ss [FUN_EQ_THM,option_orelse_def,option_then_def,LET_DEF]  
      THEN REPEAT STRIP_TAC THEN Cases_on `x x'` THEN SRW_TAC [] [])
   THEN METIS_TAC [option_orelse_assoc]);
@@ -76,5 +76,6 @@ val pull_if_lemma = store_thm("pull_if_lemma",
 val if_some_lemma = store_thm("if_some_lemma",
   ``!b x (y:'a) (z:'b). (if b then SOME (z,x) else SOME (z,y)) = SOME (z,if b then x else y)``,
   Cases THEN SIMP_TAC std_ss []);
+
 
 val _ = export_theory ();
